```py
def longest_common_subsequence(word1, word2):
    n, m = len(word1), len(word2)
    dp = [[0] * (m + 1) for _ in range(n + 1)]

    for i in range(1, n + 1):
        for j in range(1, m + 1):
            if word1[i - 1] == word2[j - 1]:
                dp[i][j] = dp[i - 1][j - 1] + 1
            else:
                dp[i][j] = max(dp[i - 1][j], dp[i][j - 1])
    i, j = n,m
    lcs = []
    while i>0 and j>0:
        if word1[i-1] == word2[j-1]:
            lcs.append(word1[i-1])
            i -= 1
            j -= 1
        elif dp[i-1][j] > dp[i][j-1]:
            i-=1
        else:
            j-=1
    return "".join(reversed(lcs))

# 입력
word1 = input().strip()
word2 = input().strip()

# 출력
print(longest_common_subsequence(word1, word2))

```
